unify.v
@@ -7,6 +7,7 @@ Require Import ListSet.
 Require Import LibTactics.
 
 Require Import type coercion utils subst co_kind var tactics compose ty_kind.
+Require Import subset.
 
 Set Implicit Arguments.
 
@@ -15,14 +16,11 @@ Inductive mapping : ctxt -> coercion -> var -> type -> type -> Type :=
                                       -> mapping Si g f lhs target.
 
 Inductive substn Si : list (var * type) -> nat -> Type :=
-| nilSubst : forall n, substn Si nil n
+| nilSubst : substn Si nil 0
 | consSubst : forall g f lhs target dom n,
                 mapping Si g f lhs target -> 
                 substn Si dom n ->
-                substn Si ((f, lhs) :: dom) (n + size_of_co false g).
-
-Definition domelt_eq_decide (d1 d2 : var * type) : decide (d1 = d2) :=
-  tuple_eq_decide var_eq_decide type_eq_decide d1 d2.
+                substn Si ((f, lhs) :: dom) (n + size_of_co g).
 
 Lemma push_domelt_eq : forall A f ty (a b : A),
   (if domelt_eq_decide (f,ty) (f,ty)
@@ -127,9 +125,20 @@ Proof.
   induction t; intros; simpl; destruct_if; auto.
 Qed.
 
+Lemma apply1_size0 : forall t Si g f ty ty2 (m : mapping Si g f ty ty2),
+  size_of_co g = 0 ->
+  apply1 m t = t.
+Proof.
+  induction t; intros; simpl; destruct_if; auto.
+  - destruct_if. eapply size0_refl in H. apply C in H. contradiction.
+    destruct m. eassumption. auto.
+  - rewrite IHt1; auto. rewrite IHt2; auto. 
+  - rewrite IHt1; auto. rewrite IHt2; auto.
+Qed.
+
 Fixpoint apply_w Si dom n (subst : substn Si dom n) (t : wrapped_type) : wrapped_type :=
   match subst with
-    | nilSubst _ => t
+    | nilSubst => t
     | consSubst _ _ _ _ _ _ mx rest => apply1 mx (apply_w rest t)
   end.
 
@@ -148,6 +157,14 @@ Proof.
   end; simpl in IHsub; rewrite IHsub; simpl; destruct_if; auto.
   generalize (mkMapping c). rewrite <- C. intro m. repeat rewrite apply1_refl. auto.
   generalize (mkMapping c). rewrite <- C. intro m. repeat rewrite apply1_refl. auto.
+Qed.
+
+Lemma apply_w_size0 : forall Si dom (w_empty : substn Si dom 0) t,
+  apply_w w_empty t = t.
+Proof.
+  intros. remember 0. induction w_empty.
+  - reflexivity.
+  - simpl. rewrite IHw_empty. apply apply1_size0. omega. omega.
 Qed.
 
 Ltac is_bare_type t :=
@@ -207,31 +224,7 @@ Proof.
     - auto.
 Qed.
 
-Inductive InT A : A -> list A -> Type :=
-| InHere : forall h t, InT h (h :: t)
-| InThere : forall a h t, InT a t -> InT a (h :: t).
-
-Lemma InT__In : forall A (a : A) (l : list A),
-  InT a l -> In a l.
-Proof.
-  induction l; intros.
-  - inverts X.
-  - inverts X. constructor. auto. apply in_cons. auto.
-Qed.
-
 Lemma in_yank_dom : forall dom f ty f' ty',
-  InT (f,ty) (yank_dom f' ty' dom) -> InT (f,ty) dom.
-Proof.
-  induction dom; intros.
-  - simpl in H. auto.
-  - simpl in H. destruct a. destruct (domelt_eq_decide (f,ty) (v,t)).
-    * inverts e. constructor.
-    * constructor. destruct (domelt_eq_decide (f',ty') (v,t)).
-      + auto.
-      + eapply IHdom. inversion H. subst. not_equal. eauto.
-Qed.
-
-Lemma in_yank_dom_P : forall dom f ty f' ty',
   In (f,ty) (yank_dom f' ty' dom) -> In (f,ty) dom.
 Proof.
   induction dom; intros.
@@ -252,32 +245,39 @@ Proof.
   - inverts H. destruct a. destruct (domelt_eq_decide (f,ty) (v,t)).
     * inverts e. rewrite yank_dom_head. auto.
     * rewrite yank_dom_tail; auto. constructor. intro Hcon.
-      apply in_yank_dom_P in Hcon. contradiction.
+      apply in_yank_dom in Hcon. contradiction.
       apply IHdom. assumption.
 Qed.
 
 Lemma yank_dom_removes : forall dom f ty,
   NoDup dom ->
-  InT (f,ty) (yank_dom f ty dom) -> False.
+  In (f,ty) (yank_dom f ty dom) -> False.
 Proof.
   induction dom; intros.
   - simpl in H0. inverts H0.
   - specialize (IHdom f ty). lapplies IHdom. contradiction.
     * simpl in H0. destruct a. destruct_if.
-      + exfalso. inverts H. apply InT__In in H0. inverts C. contradiction.
-      + inverts H0. not_equal. auto.
+      + exfalso. inverts H. inverts C. contradiction.
+      + apply in_inv in H0. inverts H0. rewrite H1 in C. not_equal. auto.
     * inverts H. auto.
 Qed.
 
-Definition yank_mapping Si dom n f ty (w : substn Si dom n) :
-  InT (f, ty) dom ->
+Lemma in_neq : forall A (a h : A) (t : list A),
+  In a (h :: t) -> a <> h -> In a t.
+Proof.
+  intros. inverts H.
+  - not_equal.
+  - auto.
+Qed.
+
+Definition yank_mapping Si dom n f ty (w : substn Si dom n)
+  (HIn : In (f, ty) dom) :
   { g : coercion &
   { target : type &
   { n' : nat &
   { (mx, w') : (mapping Si g f ty target * substn Si (yank_dom f ty dom) n') |
-    (n' + size_of_co false g = n /\
+    (n' + size_of_co g = n /\
      forall t, apply_w w t = apply1 mx (apply_w w' t)) }}}}.
-  intro HIn.
   induction w as [ ? | ? f1 ty1 ? ? ? mx rest ].
   - (* nil *) inversion HIn.
   - (* cons *) destruct (domelt_eq_decide (f1,ty1) (f,ty)) as [ Heq | Hneq ].
@@ -286,113 +286,150 @@ Definition yank_mapping Si dom n f ty (w : substn Si dom n) :
                   rewrite yank_dom_head.
                   exists (mx, rest).
                   auto.
-    * (* not equal *) inversion HIn. 
-      + (* InHere *) subst. not_equal.
-      + (* InThere *) apply IHrest in H1.
-                      destruct H1 as [g1 [target1 [n1 [[mx1 w1] pf]]]].
-                      exists g1. exists target1. exists (n1 + size_of_co false g).
-                      rewrite yank_dom_tail by auto.
-                      exists (mx1, consSubst mx w1).
-                      inverts pf.
-                      split. omega.
-  intros. simpl. rewrite H3. apply apply1_commutes_self. assumption.
+    * (* not equal *) apply in_neq in HIn; auto.
+      apply IHrest in HIn.
+      destruct HIn as [g1 [target1 [n1 [[mx1 w1] pf]]]].
+      exists g1. exists target1. exists (n1 + size_of_co g).
+      rewrite yank_dom_tail by auto.
+      exists (mx1, consSubst mx w1).
+      inverts pf.
+      split. omega.
+  intros. simpl. rewrite H0. apply apply1_commutes_self. assumption.
 Qed.
 
-Fixpoint InT_decide {A} (a : A) (l : list A) :
-  (forall (a1 a2 : A), decide (a1 = a2)) ->
-  (InT a l) + {InT a l -> False}.
+Lemma subset_yank_dom : forall f ty dom1 dom2,
+  subset (yank_dom f ty dom1) dom2 -> subset dom1 ((f,ty)::dom2).
 Proof.
-  intro Hdec_eq.
-  refine (match l with
-            | nil => inright _
-            | b :: rest => if Hdec_eq a b then inleft _ else
-                             if InT_decide A a rest Hdec_eq then inleft _ else inright _
-          end).
-  intro Hcon. inversion Hcon.
-  subst. constructor.
-  constructor. auto.
-  intro Hcon. inversion Hcon. subst. not_equal. apply _H0 in X. contradiction.
+  (* This is a terrible proof. I'm ashamed. Please fix. *)
+  unfolds subset. induction dom1; intros.
+  - inverts H0.
+  - destruct (domelt_eq_decide (f,ty) domelt).
+    * rewrite e. apply in_eq.
+    * destruct (domelt_eq_decide a domelt).
+      + subst. apply in_cons. apply H. destruct domelt. rewrite yank_dom_tail.
+        apply in_eq. auto.
+      + apply IHdom1. intros. apply H. destruct (domelt_eq_decide (f,ty) a).
+          rewrite <- e. rewrite yank_dom_head. destruct domelt0.
+          eapply in_yank_dom. eassumption. destruct a. rewrite yank_dom_tail by auto.
+          apply in_cons. assumption. apply in_inv in H0. inverts H0. not_equal.
+          assumption.
+Qed.
+
+Lemma subset_yank_dom_2 : forall f ty dom1 dom2,
+  NoDup dom1 ->
+  subset dom1 ((f,ty)::dom2) -> subset (yank_dom f ty dom1) dom2.
+Proof.
+  intros. induction dom1.
+  - simpl. apply subset_nil.
+  - simpl. destruct a. destruct_if.
+    * rewrite C in H0. rewrite <- subset_cons in H0. auto. inverts H. auto.
+    * apply subset_cons1 in H0. inverts H0. apply IHdom1 in H1.
+      apply subset_in. apply in_inv in H2. inverts H2. contradiction. auto. auto.
+      inverts H. auto.
 Qed.
 
 Unset Implicit Arguments.
-Obligation Tactic := idtac.
+Obligation Tactic := program_simpl.
 Program Fixpoint fix_dom Si dom1 n (w : substn Si dom1 n)
                            dom2 n2 (w2 : substn Si dom2 n2)
-  (HNoDup : NoDup dom1)
-  (HIn : forall f ty, InT (f,ty) dom1 -> InT (f,ty) dom2)
-  : { w_res : substn Si dom2 n | forall t, apply_w w t = apply_w w_res t } :=
+  (HNoDup1 : NoDup dom1) (HNoDup2 : NoDup dom2)
+  : { dom : list (var * type) &
+    { w1' : substn Si dom n |
+      (forall t, apply_w w1' t = apply_w w t) /\
+      subset dom1 dom /\ subset dom2 dom /\ (subset dom1 dom2 -> dom = dom2) /\
+      (forall domelt, In domelt dom -> (In domelt dom1 \/ In domelt dom2)) /\
+      NoDup dom }} :=
   match w2 with
-    | nilSubst _ => nilSubst _ _
+    | nilSubst => existT _ dom1 w
     | consSubst _ f1 ty1 _ rest _ _ w2' =>
-      match InT_decide (f1,ty1) dom1 domelt_eq_decide with
-        | inleft HInT =>
-          let sig_mapping := projT2 (projT2 (projT2 (yank_mapping w HInT))) in
-          consSubst (fst (proj1_sig sig_mapping)) (fix_dom _ _ _ (snd (proj1_sig sig_mapping)) _ _ w2' _ _)
-        | inright Hcon =>
+      match in_dec domelt_eq_decide (f1,ty1) dom1 with
+        | left HIn =>
+          let yanked := yank_mapping f1 ty1 w HIn in
+          match yanked with
+            | existT _ (existT _ (existT _ (exist (mx, w1') _))) =>
+          let fixed :=  fix_dom _ _ _ w1' _ _ w2' _ _ in
+          match fixed with
+            | existT dom fixed_w =>
+          existT _ ((f1,ty1)::dom) (consSubst mx fixed_w)
+          end end
+        | right Hcon =>
           let t := TFun f1 ty1 in
           let k_w_proof := typeKind Si t _ in
-          consSubst (mkMapping (CKRefl (proj2_sig k_w_proof)))
-                    (fix_dom _ _ _ w _ _ w2' _ _)
+          let fixed := fix_dom _ _ _ w _ _ w2' _ _ in
+          match fixed with
+            | existT dom fixed_w =>
+          existT _ ((f1,ty1)::dom) (consSubst (mkMapping (@CKRefl _ _ k_w_proof _)) fixed_w)
+          end
       end
   end.
-Require Import Tactics.
+
 Next Obligation.
-  program_simpl.
-  assert (dom1 = []). { destruct dom1. auto. destruct p. specialize (HIn v t0).
-                        lapplies HIn. inverts H. constructor. }
-  destruct w.
-    - reflexivity.
-    - discriminate.
+  repeat split.
+  - apply subset_refl.
+  - apply subset_nil.
+  - intro. destruct dom1.
+    * auto.
+    * unfolds subset. specialize (H p). lapplies H. inverts H0. apply in_eq.
+  - intros. tauto.
+  - assumption.
 Qed.
 
 Next Obligation.
-  intros.
-  apply no_dup_yank_dom. assumption.
+  clear Heq_yanked.
+  apply no_dup_yank_dom. auto.
 Qed.
 
 Next Obligation.
-  program_simpl.
-  pose proof H as Hyank. apply in_yank_dom in H. apply HIn in H. inverts H.
-  - apply yank_dom_removes in Hyank; auto. contradiction.
-  - auto.
+  inverts HNoDup2. auto.
 Qed.
 
 Next Obligation.
-  program_simpl. generalize (yank_mapping w HInT). intro s. destruct s. destruct s.
-  destruct s. simpl. pose proof (proj2_sig s). simpl in H. destruct s. simpls.
-  destruct x2. tauto.
-Qed.
+    repeat split.
+  - intros. squash_eq_rect. rewrite e0. rewrite e1.
+    reflexivity.
 
-Ltac squash_eq_rect :=
-  let H := fresh in
-  match goal with
-    | [ |- context[eq_rect _ _ _ _ ?Heq] ] => generalize Heq; intro H; destruct H; simpl
-  end.
-
-Next Obligation.
-  intros. squash_eq_rect. destruct sig_mapping. destruct x. simpl. abstract_sig.
-  rewrite <- H0. inversion y. apply H2.
+  - clear Heq_fixed Heq_yanked. apply subset_yank_dom. assumption.
+  - clear Heq_fixed Heq_yanked. apply subset_cons. inverts HNoDup2. auto. assumption.
+  - clear Heq_fixed Heq_yanked. intros. f_equal. apply e2.
+    apply subset_yank_dom_2. assumption. assumption.
+  - clear Heq_fixed Heq_yanked. intros. inverts H.
+    * tauto.
+    * apply o in H0. inverts H0.
+      + destruct domelt. apply in_yank_dom in H. tauto.
+      + tauto.
+  - clear Heq_fixed Heq_yanked. constructor; auto. intro Hcon.
+    apply o in Hcon. inverts Hcon.
+    * apply yank_dom_removes in H. auto. auto.
+    * inverts HNoDup2. contradiction.
 Defined.
 
-Obligation Tactic := program_simpl.
-
 Next Obligation.
-  clear Heq_w2. inverts w2. inverts X. apply co_kind_reg_t1 in H0. assumption.
+  clear Heq_w2. inverts wildcard'2. apply co_kind_reg_t1 in H. auto.
 Qed.
 
 Next Obligation.
-  pose proof H as Hcopy. apply HIn in H. inverts H. 
-  - contradiction.
-  - auto.
+  inverts HNoDup2. auto.
 Qed.
 
 Next Obligation.
-  squash_eq_rect.
-  match goal with
-    | [ |- context[mkMapping ?garbage] ] => generalize garbage
-  end.
-  intro c. generalize (mkMapping c). intro m.
-  rewrite apply1_refl. apply e.
+  abstract_sig. auto.
+Defined.
+
+Next Obligation.
+  repeat split; try clear Heq_fixed.
+  - squash_eq_rect. intro.
+    match goal with
+      | [ |- context[apply1 ?garbage _] ] => generalize garbage
+    end. intro.
+    clear Heq_fixed. rewrite e. apply apply1_refl.
+
+  - apply subset_cons2. assumption.
+  - apply subset_cons. inverts HNoDup2. assumption. assumption.
+  - intro. f_equal. apply e0. eapply subset_neq. apply Hcon. assumption.
+  - intros. inverts H. tauto. apply o in H0. inverts H0; tauto.
+  - constructor; auto. intro. apply o in H. inverts H.
+    * contradiction.
+    * inverts HNoDup2. contradiction.
 Defined.
 
 Arguments fix_dom [_ _ _] _ [_ _] _ _ _.
