subset.v
@@ -1,0 +1,78 @@
+Require Import LibVar.
+Require Import LibTactics.
+Require Import List.
+
+Require Import type utils var.
+
+Set Implicit Arguments.
+
+Definition domelt_eq_decide (d1 d2 : var * type) : decide (d1 = d2) :=
+  tuple_eq_decide var_eq_decide type_eq_decide d1 d2.
+
+Definition subset (dom1 dom2 : list (var * type)) : Prop :=
+  forall domelt, In domelt dom1 -> In domelt dom2.
+
+Lemma subset_refl : forall s,
+  subset s s.
+Proof.
+  intros. intro. auto.
+Qed.
+
+Lemma subset_nil : forall (s : list (var * type)),
+  subset nil s.
+Proof.
+  unfold subset. introv H. inverts H.
+Qed.
+
+Lemma subset_cons1 : forall d s1 s2,
+  subset (d::s1) s2 -> (subset s1 s2 /\ In d s2).
+Proof.
+  unfold subset; intros; repeat split; intros.
+  - apply H. apply in_cons. auto.
+  - apply H. apply in_eq.
+Qed.
+
+Lemma subset_cons2 : forall d s1 s2,
+  subset s1 s2 -> subset s1 (d::s2).
+Proof.
+  unfold subset; intros. apply in_cons. auto.
+Qed.
+
+Lemma subset_in : forall d s1 s2,
+  In d s2 -> 
+  subset s1 s2 ->
+  subset (d::s1) s2.
+Proof.
+  unfold subset; intros.
+  destruct (domelt_eq_decide d domelt).
+   - subst. auto.
+   - apply H0. apply in_inv in H1. inversion H1. contradiction. auto.
+Qed.
+
+Lemma subset_cons : forall d s1 s2,
+  ~ In d s1 ->
+  (subset s1 s2 <-> subset (d::s1) (d::s2)).
+Proof.
+  unfold subset; intros; split; intros.
+  * apply in_inv in H1. inversion H1.
+    - rewrite H2. apply in_eq.
+    - apply in_cons. apply H0. assumption.
+  * pose proof H1 as HIn.
+    eapply in_cons in H1. apply H0 in H1. apply in_inv in H1. inversion H1.
+    - subst. contradiction.
+    - auto.
+Qed.
+
+Lemma subset_neq : forall d s1 s2,
+  ~ In d s1 ->
+  subset s1 (d::s2) ->
+  subset s1 s2.
+Proof.
+  intros; induction s1.
+  - apply subset_nil.
+  - apply subset_in. unfold subset in H0. assert (In a (a :: s1)) by apply in_eq.
+    apply H0 in H1. apply in_inv in H1. inversion H1. subst.
+    assert (In a (a :: s1)) by apply in_eq. contradiction. assumption.
+    apply IHs1. intro Hcon. eapply in_cons in Hcon. apply H in Hcon. auto.
+    eapply subset_cons1. eassumption.
+Qed.
